RL.v
@@ -395,12 +395,12 @@ Proof with (fold'; try abbrv).
   have ndind: NoDup ind by exact/sorted_nodup.
   xin (1,0): (xwp;xapp=> ans); (xwp;xapp=> iX); 
     (xwp;xapp=> iY); (xwp;xapp=> step)...
-  have xind_notnil : xind <> nil by destruct xind; try discriminate; simpl in *; try math.
-  have yind_notnil : yind <> nil by destruct yind; try discriminate; simpl in *; try math.
+  have xind_notnil : xind <> nil by apply notnil_length; try math.
+  have yind_notnil : yind <> nil by apply notnil_length; try math.
   have maxxindE: max xind = N by rewrite -(sorted_max_size _ (i:=Mx)) //; try math.
   have maxyindE: max yind = N by rewrite -(sorted_max_size _ (i:=My)) //; try math.
   have maxindE: max ind = N by rewrite max_merge //; try math.
-  rewrite (@interval_unionE ind)=> //.
+  rewrite (@interval_unionE ind) // ?merge_nth0; try math.
   set (Inv (b : bool) (i : int) := 
     arr(x_ind, xind)⟨1, 0⟩ \* arr(y_ind, yind)⟨1, 0⟩ \\*
     arr(x_val, xval)⟨1, 0⟩ \* arr(y_val, yval)⟨1, 0⟩ \\*
@@ -440,7 +440,7 @@ Proof with (fold'; try abbrv).
       move: (indL); rewrite {1}indE {1}ENy {1}C Z.min_id.
       move/(sorted_le_rev yxind)=> ?.
       have indlE: ind[l+1] = Z.min xind[ix + 1] yind[iy + 1].
-      { rewrite merge_nthS -/ind ?indE...
+      { rewrite (merge_nthS (def:=N)) -/ind ?indE...
         rewrite -{1}C Z.min_id {2}C Z.min_id ?search_nth... }
       rewrite /R2/R3.
       xin (2,0): xapp (@get_spec xind xval HindIIL ix)...
@@ -466,9 +466,9 @@ Proof with (fold'; try abbrv).
       { apply/(sorted_le_rev yxind)...
         suff: xind[ix] >= 0 by lia. exact/IILG0. } 
       have indlE: ind[l+1] = Z.min xind[ix + 1] yind[iy].
-      { rewrite merge_nthS -/ind ?indE...
+      { rewrite (merge_nthS (def:=N)) -/ind ?indE...
         rewrite (Z.min_l xind[ix]) ?search_nth...
-        rewrite (@search_nth_pred _ iy)... }
+        rewrite (@search_nth_pred N _ iy)... }
       rewrite /R2/R3.
       xin (2,0): xapp (@get_spec xind xval HindIIL ix)...
       { move=> [>]; indomE=>-[?]/=; lia. }
@@ -493,9 +493,9 @@ Proof with (fold'; try abbrv).
     { apply/(sorted_le_rev sxind)...
       suff: yind[iy] >= 0 by lia. exact/IILG0. } 
     have indlE: ind[l+1] = Z.min xind[ix] yind[iy + 1].
-    { rewrite merge_nthS -/ind ?indE...
+    { rewrite (merge_nthS (def:=N)) -/ind ?indE...
       rewrite (Z.min_r xind[ix]) ?search_nth...
-      rewrite (@search_nth_pred _ ix)... }
+      rewrite (@search_nth_pred N _ ix)... }
     rewrite /R2/R3.
     xin (2,0): xapp (@get_spec xind xval HindIIL (ix-1))...
     { move=> [>]; indomE=>-[?]/=;
